Rename VSU components

theories/Int63/vst/spec/spec.v
@@ -301,27 +301,29 @@ Definition int63_not_spec: ident * funspec :=
       SEP ( ).
 
 Module int63__specs.
+  Definition exports: funspecs :=
+    [ decode_int63_spec
+    ; encode_int63_spec
+    ; int63_zero_spec
+    ; int63_one_spec
+    ; int63_neg_spec
+    ; int63_abs_spec
+    ; int63_add_spec
+    ; int63_sub_spec
+    ; int63_mul_spec
+    ; int63_div_spec
+    ; int63_rem_spec
+    ; int63_shiftl_spec
+    ; int63_shiftr_spec
+    ; int63_or_spec
+    ; int63_and_spec
+    ; int63_xor_spec
+    ; int63_not_spec
+  ].
   Definition externs: funspecs := [].
   Definition imports: funspecs := [].
-  Definition internals: funspecs := [].
-  Definition exports: funspecs := [
-    decode_int63_spec;
-    encode_int63_spec;
-    int63_zero_spec;
-    int63_one_spec;
-    int63_neg_spec;
-    int63_abs_spec;
-    int63_add_spec;
-    int63_sub_spec;
-    int63_mul_spec;
-    int63_div_spec;
-    int63_rem_spec;
-    int63_shiftl_spec;
-    int63_shiftr_spec;
-    int63_or_spec;
-    int63_and_spec;
-    int63_xor_spec;
-    int63_not_spec
-  ].
-  Definition all: funspecs := imports ++ internals ++ exports.
+  Definition private: funspecs := [].
+  Definition internals: funspecs := private ++ exports.
+  Definition gprog: funspecs := imports ++ internals.
+  Definition vprog: varspecs := ltac:(mk_varspecs prog).
 End int63__specs.
